\documentclass[12pt]{article}
\usepackage{amsmath}
\usepackage{ amssymb }
\usepackage{breqn}
\begin{document}

\title{SWW soliton}
\author{Jordan Pitt / u5013521}

\section{SWW soliton}
The continuity equation is:
\begin{equation}
\label{coneq1}
h_t + uh_x + u_xh = 0
\end{equation}

the momentum equation is
\[\left(uh\right)_t + \left(u^2h + g\frac{h^2}{2}\right)_x = 0\]
expanding

\[u_th + uh_t + \left(u^2h\right)_x + ghh_x = 0\]

\[u_th + uh_t + 2uu_xh + u^2h_x  + ghh_x = 0\]

using \eqref{coneq1}

\[u_th - u^2h_x - uu_xh  + 2uu_xh + u^2h_x  + ghh_x = 0\]

\[u_th + uu_xh  + ghh_x = 0\]
when $h > 0$
\begin{equation}
\label{veleq1}
u_t + uu_x  + gh_x = 0
\end{equation}

want solutions to \eqref{coneq1} and \eqref{veleq1} such that

\[h(x,t) = \phi(y) ,\quad y = x -ct\]
\[u(x,t) = \psi(y) ,\quad y = x -ct\]

Substituting these into \eqref{coneq1} gives
\[-c\phi'(y) + \psi(y)\phi'(y) + \psi'(y)\phi(y) = 0\]

\[ \left[\psi(y) - c\right]\phi'(y) + \psi'(y)\phi(y) = 0\]
\begin{equation}
\label{eq1}
\left[\psi(y) - c\right]\phi'(y) + \psi'(y)\phi(y) = 0
\end{equation}

Substituting these into \eqref{veleq1} gives
\[-c\psi'(y) + \psi(y)\psi'(y)  + g\phi'(y) = 0\]

\[\left[\psi(y) -c\right]\psi'(y) + g\phi'(y) = 0\]
\begin{equation}
\label{eq2}
\left[\psi(y) -c\right]\psi'(y) + g\phi'(y) = 0
\end{equation}

Rearranging \eqref{eq2} we get:

\[\left[\psi(y) -c\right]\psi'(y) = - g\phi'(y)\]
\[\left[\psi(y) -c\right] = \frac{- g\phi'(y)}{\psi'(y)}\]

subbing into \eqref{eq1}:

\[\frac{- g\phi'(y)}{\psi'(y)}\phi'(y) + \psi'(y)\phi(y) = 0\]

\[\left(\psi'(y)\right)^2\phi(y) =g \left(\phi'(y)\right)^2\]

\[\psi'(y)= \sqrt{g}\frac{\phi'(y)}{\sqrt{\phi(y)} }\]

In particular since $(\sqrt{f(x)})' = f(x)f^{-1/2}(x)$ we must have

\[\psi(y)= \sqrt{g}\sqrt{\phi(y)}  + D\]

\[u(x,t)= \sqrt{g}\sqrt{h(x,t)}  + D\]









\end{document}
