\documentclass[12pt]{article}
\usepackage{amsmath}
\usepackage{ amssymb }
\usepackage{breqn}
\begin{document}

\title{G for soliton}
\author{Jordan Pitt / u5013521}

\section{Cell Averaged G}
We have a quartic:

\[Q_j(x) = a_j(x - x_j)^4 + b_j(x - x_j)^3 + c_j(x - x_j)^2 + d_j(x - x_j) + e_j\]

Satisfying the equations
\[Q_j(x_j) = q_j\]
\[Q_j(x_{j+1}) = q_{j+1}\]
\[Q_j(x_{j+2}) = q_{j+2}\]
\[Q_j(x_{j-1}) = q_{j-1}\]
\[Q_j(x_{j-2}) = q_{j-2}\]

In particular we have that

\begin{equation}
\label{e}
q_j = e_j
\end{equation}

\begin{equation}
\label{1}
q_{j+1} = a_j(\Delta x)^4 + b_j(\Delta x)^3 + c_j(\Delta x)^2 + d_j(\Delta x) + e_j
\end{equation}

\begin{equation}
\label{2}
q_{j+2} = 16a_j(\Delta x)^4 + 8b_j(\Delta x)^3 + 4c_j(\Delta x)^2 + 2d_j(\Delta x) + e_j
\end{equation}

\begin{equation}
\label{3}
q_{j-1} = a_j(\Delta x)^4 - b_j(\Delta x)^3 + c_j(\Delta x)^2 - d_j(\Delta x) + e_j
\end{equation}

\begin{equation}
\label{4}
q_{j-2} = 16a_j(\Delta x)^4 - 8b_j(\Delta x)^3 + 4c_j(\Delta x)^2 - 2d_j(\Delta x) + e_j
\end{equation}

Adding \eqref{1} and \eqref{3} gives
\begin{equation}
\label{5}
q_{j+1} + q_{j-1} = 2a_j(\Delta x)^4 + 2c_j(\Delta x)^2 + 2q_j
\end{equation}
Adding \eqref{2} and \eqref{4} gives
\begin{equation}
\label{6}
q_{j+2} + q_{j-2} = 32a_j(\Delta x)^4 + 8c_j(\Delta x)^2 + 2q_j
\end{equation}

\eqref{6} - 4 $\times$ \eqref{5}:
\[q_{j+2} + q_{j-2} -4q_{j+1} -4q_{j-1} = 24a_j(\Delta x)^4 - 6q_j\]
\[q_{j+2} -4q_{j+1} + 6q_j -4q_{j-1}  + q_{j-2} = 24a_j(\Delta x)^4 \]

\begin{equation}
\label{a}
a_j = \frac{q_{j+2} -4q_{j+1} + 6q_j -4q_{j-1}  + q_{j-2}}{24 \Delta x^4 }
\end{equation}

Subbing the known values into \eqref{5} gives
\[q_{j+1} + q_{j-1} = 2\frac{q_{j+2} -4q_{j+1} + 6q_j -4q_{j-1}  + q_{j-2}}{24 \Delta x^4 }(\Delta x)^4 + 2c_j(\Delta x)^2 + 2q_j\]

\[q_{j+1} + q_{j-1} = \frac{q_{j+2} -4q_{j+1} + 6q_j -4q_{j-1}  + q_{j-2}}{12 } + 2c_j(\Delta x)^2 + 2q_j\]

\[q_{j+1} + q_{j-1} - 2q_j +  \frac{-q_{j+2} +4q_{j+1} - 6q_j +4q_{j-1}  - q_{j-2}}{12 } = 2c_j(\Delta x)^2\]

\[\frac{12q_{j+1} + 12q_{j-1} - 24q_j -q_{j+2} +4q_{j+1} - 6q_j +4q_{j-1}  - q_{j-2}}{12 } = 2c_j(\Delta x)^2\]

\[\frac{-q_{j+2} +16q_{j+1} - 30q_j + 16q_{j-1}  - q_{j-2}}{12 } = 2c_j(\Delta x)^2\]

\begin{equation}
\label{c}
c_j = \frac{-q_{j+2} +16q_{j+1} - 30q_j + 16q_{j-1}  - q_{j-2}}{24 \Delta x^2 }
\end{equation}

Subtracting \eqref{3} from \eqref{1} gives
\begin{equation}
\label{7}
q_{j+1} - q_{j-1} = 2b_j(\Delta x)^3 + 2d_j(\Delta x)
\end{equation}

Subtracting \eqref{4} from \eqref{2} gives
\begin{equation}
\label{8}
q_{j+2} - q_{j-2}  = 16b_j(\Delta x)^3 + 4d_j(\Delta x)
\end{equation}

\eqref{8} - 2 $\times$ \eqref{7}:
\[q_{j+2} - q_{j-2} - 2q_{j+1} + 2q_{j-1} = 12b_j(\Delta x)^3\]

\begin{equation}
\label{b}
b_j = \frac{q_{j+2} - 2q_{j+1} + 2q_{j-1} - q_{j-2}}{12 \Delta x^3 }
\end{equation}

Subbing the known values in to  \eqref{7} gives

\[q_{j+1} - q_{j-1} = \frac{q_{j+2} - 2q_{j+1} - q_{j-2} + 2q_{j-1}}{6} + 2d_j(\Delta x) \]

\[q_{j+1} - q_{j-1} + \frac{-q_{j+2} + 2q_{j+1} + q_{j-2} - 2q_{j-1}}{6} = + 2d_j(\Delta x) \]

\[\frac{6q_{j+1} - 6q_{j-1}  -q_{j+2} + 2q_{j+1} + q_{j-2} - 2q_{j-1}}{6} = 2d_j(\Delta x) \]

\[\frac{-q_{j+2} + 8q_{j+1} - 8q_{j-1} + q_{j-2}}{6} = 2d_j(\Delta x) \]

\begin{equation}
\label{d}
d_j = \frac{-q_{j+2} + 8q_{j+1} - 8q_{j-1} + q_{j-2}}{12\Delta x}
\end{equation}

So to recall we have 
\[a_j = \frac{q_{j+2} -4q_{j+1} + 6q_j -4q_{j-1}  + q_{j-2}}{24 \Delta x^4 }\]
\[b_j = \frac{q_{j+2} - 2q_{j+1} + 2q_{j-1} - q_{j-2}}{12 \Delta x^3 }\]
\[c_j = \frac{-q_{j+2} +16q_{j+1} - 30q_j + 16q_{j-1}  - q_{j-2}}{24 \Delta x^2 }\]
\[d_j = \frac{-q_{j+2} + 8q_{j+1} - 8q_{j-1} + q_{j-2}}{12\Delta x}\]
\[e_j = q_j\]

test this for  $Q_j(x_{j+1}) = q_{j+1}$

\begin{equation*}
\begin{split}
\frac{q_{j+2} -4q_{j+1} + 6q_j -4q_{j-1}  + q_{j-2}}{24 \Delta x^4 }(\Delta x)^4 + \frac{q_{j+2} - 2q_{j+1} + 2q_{j-1} - q_{j-2}}{12 \Delta x^3 }(\Delta x)^3  \\ + \frac{-q_{j+2} +16q_{j+1} - 30q_j + 16q_{j-1}  - q_{j-2}}{24 \Delta x^2 }(\Delta x)^2 + \frac{-q_{j+2} + 8q_{j+1} - 8q_{j-1} + q_{j-2}}{12\Delta x}(\Delta x) + q_j
\end{split}
\end{equation*}
\begin{equation*}
\begin{split}
=\frac{q_{j+2} -4q_{j+1} + 6q_j -4q_{j-1}  + q_{j-2}}{24} + \frac{q_{j+2} - 2q_{j+1} + 2q_{j-1} - q_{j-2}}{12} \\ + \frac{-q_{j+2} +16q_{j+1} - 30q_j + 16q_{j-1}  - q_{j-2}}{24} + \frac{-q_{j+2} + 8q_{j+1} - 8q_{j-1} + q_{j-2}}{12} + q_j
\end{split}
\end{equation*}

\begin{equation*}
\begin{split}
=\frac{q_{j+2} -4q_{j+1} + 6q_j -4q_{j-1}  + q_{j-2}}{24} + \frac{2q_{j+2} - 4q_{j+1} + 4q_{j-1} - 2q_{j-2}}{24} \\ + \frac{-q_{j+2} +16q_{j+1} - 30q_j + 16q_{j-1}  - q_{j-2}}{24} + \frac{-2q_{j+2} + 16q_{j+1} - 16q_{j-1} + 2q_{j-2}}{24} + q_j
\end{split}
\end{equation*}

\begin{equation*}
=\frac{24q_{j+1}}{24} = q_{j+1} \square
\end{equation*}



\end{document}


